theories/examples/stack_helping/stack.v
@@ -87,7 +87,7 @@ Definition offerRegR :=
   gmapUR loc (agreeR (prodO valO (prodO gnameO ref_idO))).
 
 Class offerRegPreG Σ := OfferRegPreG {
-  offerReg_inG :> inG Σ (authR offerRegR)
+  offerReg_inG :: inG Σ (authR offerRegR)
 }.
 
 Definition offerize (x : (val * gname * ref_id)) :
