theories/lib/lock.v
@@ -15,7 +15,7 @@ Definition with_lock : val := λ: "e" "l" "x",
   let: "v" := "e" "x" in
   release "l";; "v".
 
-Class lockG Σ := LockG { lock_tokG :> inG Σ (exclR unitO) }.
+Class lockG Σ := LockG { lock_tokG :: inG Σ (exclR unitO) }.
 Definition lockΣ : gFunctors := #[GFunctor (exclR unitO)].
 
 Global Instance subG_lockΣ {Σ} : subG lockΣ Σ → lockG Σ.
