theories/logic/adequacy.v
@@ -6,8 +6,8 @@ From iris.heap_lang Require Export adequacy.
 From reloc.logic Require Export spec_ra model.
 
 Class relocPreG Σ := RelocPreG {
-  reloc_preG_heap :> heapGpreS Σ;
-  reloc_preG_cfg  :> inG Σ (authR cfgUR)
+  reloc_preG_heap :: heapGpreS Σ;
+  reloc_preG_cfg  :: inG Σ (authR cfgUR)
 }.
 
 Definition relocΣ : gFunctors := #[heapΣ; GFunctor (authR cfgUR)].
